some wrong attempt

HoareFunc.v
@@ -60,6 +60,24 @@ End Simple.
 
 Module Axiomatic.
 
+(* ceval' sigma c st1 st2
+
+sg n
+0 => _ _ _ => False
+S n => ceval' (sg n)
+
+sigma
+exists n, sg n
+
+ceval' sigma <-> ceval
+
+Delta P f Q -> Delta |-- P f Q -> Delta |-- P c Q -> |== P c Q *)
+
+Definition assn_sub (P : Assertion) (X : var) (a : aexp) : Assertion :=
+  fun st => P (update_state st X (aeval st a)).
+
+Notation "P [ X |-> a ]" := (assn_sub P X a) (at level 10, X at next level).
+
 Inductive hoare_triple : Type :=
   | Build_hoare_triple (P : Assertion) (c : com) (Q : Assertion).
 
@@ -67,12 +85,40 @@ Notation "{{ P }}  c  {{ Q }}" :=
   (Build_hoare_triple P c Q) (at level 90, c at next level).
 
 Inductive provable (fc : func_context) (lf : public_funcs) (fp : func_predicate) : hoare_triple -> Prop :=
+  (* fixed reentry *)
   | hoare_reentry : forall P I,
-        localp P ->
-        globalp I ->
-        (forall f, In f lf ->
-          In (I, I) (fp f)) ->
-        provable fc lf fp ({{P AND I}} CReentry {{P AND I}}).
+      localp P ->
+      globalp I ->
+      (forall f, In f lf ->
+        In (I, I) (fp f)) ->
+      provable fc lf fp ({{P AND I}} CReentry {{P AND I}})
+  (* function predicate call *)
+  | hoare_call : forall f pv P Q R,
+      globalp Q ->
+      localp R ->
+      In (P, Q) (fp f) ->
+      provable fc lf fp ({{(pv_to_assertion fc f pv P) AND R}} CCall f pv {{Q AND R}})
+  (* traditional ones *)
+  | hoare_skip : forall (P : Assertion),
+      provable fc lf fp ({{P}} CSkip {{P}})
+  | hoare_asgn_bwd : forall (P : Assertion) (X : var) (E : aexp),
+      provable fc lf fp ({{ P [ X |-> E] }} CAss X E {{ P }})
+  | hoare_seq : forall (P Q R: Assertion) (c1 c2: com),
+      provable fc lf fp ({{P}} c1 {{Q}}) ->
+      provable fc lf fp ({{Q}} c2 {{R}}) ->
+      provable fc lf fp ({{P}} c1;;c2 {{R}})
+  | hoare_if : forall (P Q : Assertion) (b : bexp) (c1 c2 : com),
+      provable fc lf fp ({{ P AND {[b]} }} c1 {{ Q }}) ->
+      provable fc lf fp ({{ P AND NOT {[b]} }} c2 {{ Q }}) ->
+      provable fc lf fp ({{ P }} If b Then c1 Else c2 EndIf {{ Q }})
+  | hoare_while_linear : forall P (b : bexp) c,
+    provable fc lf fp ({{P AND {[b]}}} c {{P}}) ->
+    provable fc lf fp ({{P}} While b Do c EndWhile {{P AND NOT {[b]}}})
+  | hoare_consequence : forall (P P' Q Q' : Assertion) c,
+      P |-- P' ->
+      provable fc lf fp ({{P'}} c {{Q'}}) ->
+      Q' |-- Q ->
+      provable fc lf fp ({{P}} c {{Q}}).
 
 Notation "fc lf fp |--  tr" := (provable fc lf fp tr) (at level 91, no associativity).
 
@@ -97,7 +143,7 @@ Definition valid (fc : func_context) (lf : public_funcs) (fp : func_predicate) (
 
 Notation "fc lf fp |== tr" := (valid fc lf fp tr) (at level 91, no associativity).
 
-
+(** Soundness *)
 Lemma reentry_sound fc lf fp :
   forall P I,
   localp P ->
@@ -124,6 +170,29 @@ Proof.
     exact H5.
 Qed.
 
+Lemma call_sound fc lf fp :
+  forall f pv P Q R,
+  globalp Q ->
+  localp R ->
+  In (P, Q) (fp f) ->
+  valid fc lf fp ({{(pv_to_assertion fc f pv P) AND R}} CCall f pv {{Q AND R}}).
+Proof.
+  unfold valid, fp_valid, triple_valid.
+  unfold andp.
+  intros.
+  inversion H4; subst.
+  destruct H11 as [loc2 ?].
+  destruct H3.
+  split.
+  - specialize (H2 _ _ _ H1).
+    unfold pv_to_assertion in H1.
+    specialize (H2 _ _ H3 H5).
+    eapply H.
+    exact H2.
+  - eapply H0.
+    exact H6.
+Qed.
+
 Theorem hoare_sound: forall fc lf fp tr,
   provable fc lf fp tr ->
   valid fc lf fp tr.
@@ -131,8 +200,60 @@ Proof.
   intros.
   induction H.
   - apply reentry_sound; assumption.
-Qed.
+  - apply call_sound; assumption.
+Admitted.
+(** [] *)
 
+
+Definition reentry_semantic fc lf (st1 st2 : state) : Prop :=
+  match st1, st2 with
+  | (loc1, glb1), (loc2, glb2) =>
+      arbitrary_eval fc lf loc1 glb1 glb2 /\ loc1 = loc2
+  end.
+
+Theorem hoare_complete : forall fc lf fp tr,
+  fp_valid fc lf fp ->
+  valid fc lf fp tr ->
+  provable fc lf fp tr.
+Proof.
+  intros.
+  destruct tr.
+  specialize (H0 H).
+  unfold triple_valid in H0.
+  induction c.
+  - admit.
+  - admit.
+  - admit.
+  - admit.
+  - admit.
+  - admit.
+  - remember ((fun st => exists st0, P st0 /\ reentry_semantic fc lf st0 st):Assertion) as I.
+    epose proof hoare_consequence _ _ _ _ I _ I _ _ _ _.
+    Unshelve.
+    + exact H1.
+    + unfold derives.
+      intros.
+      subst.
+      exists st.
+      split; [exact H1 |].
+      destruct st as (loc, glb).
+      simpl.
+      split; [constructor | auto].
+    + replace I with ((fun st => True) AND I).
+      eapply hoare_reentry.
+      * unfold localp.
+        intros. exact H1.
+      * unfold globalp.
+        subst. unfold reentry_semantic.
+        intros.
+        destruct H1 as [[loc0 glb0] [? [? ?]]].
+        subst.
+        exists (loc2, glb0). admit.
+      * admit.
+      * unfold andp.
+        admit.
+    + admit.
+Admitted.
 
 
 End Axiomatic.
